example/ttcan2/Network.TTCan.Impl.Util.fst
@@ -1,0 +1,73 @@
+module Network.TTCan.Impl.Util
+#lang-pipit
+
+open Pipit.Source
+module PSSB = Pipit.Prim.HasStream
+
+module U64     = Network.TTCan.Prim.U64
+module S32R    = Network.TTCan.Prim.S32R
+
+open Network.TTCan.Types
+
+(* One-cycle delay; on the first cycle returns the type's default value. *)
+let pre
+  (#a: eqtype) {| PSSB.has_stream a |}
+  (v: stream a)
+    : stream a =
+  PSSB.val_default `fby` v
+
+(* True when value changes; initially true *)
+let edge
+  (#a: eqtype) {| PSSB.has_stream a |}
+  (v: stream a)
+    : stream bool =
+  if true `fby` false then true else (v <> pre v)
+
+(* True when value transitions to true; initially true when v initially true *)
+let rising_edge
+  (v: stream bool)
+    : stream bool =
+  v && not (pre v)
+
+(* True when value transitions FROM true; initially false regardless of v *)
+let falling_edge
+  (v: stream bool)
+    : stream bool =
+  not v && pre v
+
+(* Check whether the value stream `v` only changes when clock `k` is true. *)
+let is_sampled_on
+  (#a: eqtype) {| PSSB.has_stream a |}
+  (v: stream a)
+  (k: stream bool)
+    : stream bool =
+  if true `fby` false then true else (v = pre v || k)
+
+(* Resettable latch. *)
+[@@derive_has_stream]
+type latch_args = { set: bool; reset: bool }
+
+let latch (args: stream latch_args): stream bool =
+  rec' (fun l ->
+    if args.set
+    then true
+    else if args.reset
+    then false
+    else pre l)
+
+(**** Time utilities ***)
+
+let local_time_valid (cfg: config) (local_time: stream ntu): stream bool =
+  let prev = pre local_time in
+  let next = U64.op_Plus prev (S32R.s32r_to_u64 cfg.triggers.ttcan_exec_period) in
+  if true `fby` false
+  then true
+  else (U64.op_Less prev local_time && U64.op_Less_Equals local_time next)
+
+let cycle_time_valid (cfg: config) (ref_ck: stream bool) (cycle_time: stream ntu): stream bool =
+  let ttcan_exec_period = S32R.s32r_to_u64 cfg.triggers.ttcan_exec_period in
+  let prev = pre cycle_time in
+  let next = U64.op_Plus prev ttcan_exec_period in
+  if (if true `fby` false then true else ref_ck)
+  then U64.op_Less cycle_time ttcan_exec_period
+  else U64.op_Less prev cycle_time && U64.op_Less_Equals cycle_time next
