example/ttcan2/Network.TTCan.Prim.S32R.fst
@@ -1,0 +1,148 @@
+(* Signed 32-bit integers with a statically-known range.
+  The range is inclusive.
+  Operations are generally saturating.
+*)
+module Network.TTCan.Prim.S32R
+
+module PSSB      = Pipit.Prim.HasStream
+
+module REPR    = FStar.Int32
+module Int     = FStar.Int
+module Cast    = FStar.Int.Cast
+module U8      = FStar.UInt8
+module U64     = FStar.UInt64
+
+module Math    = FStar.Math.Lemmas
+
+type bound = i: int { Int.fits i REPR.n }
+type bounds = { min: bound; max: max: bound { min <= max }}
+
+type t (b: bounds) = { repr: s32: REPR.t { b.min <= REPR.v s32 /\ REPR.v s32 <= b.max } }
+
+let v (#b: bounds) (r: t b): i: int { b.min <= i /\ i <= b.max } =
+  REPR.v r.repr
+
+let s32r (#b: bounds) (x: int { b.min <= x /\ x <= b.max })
+  : s: t b { v s == x } =
+  { repr = REPR.int_to_t x }
+
+// disable instance: each instance should instantiate itself
+let has_stream_S32R (b: bounds): PSSB.has_stream (t b) = {
+  ty_id = [`%t; string_of_int b.min; string_of_int b.max];
+  val_default = s32r b.min;
+}
+
+
+
+let inc_sat (#b: bounds) (x: t b)
+  : s: t b { v s >= v x /\ v s <= v x + 1 /\ (v s < b.max ==> v s = v x + 1) } =
+  if x.repr `REPR.lt` REPR.int_to_t b.max
+  then { repr = REPR.add x.repr 1l }
+  else x
+
+let dec_sat (#b: bounds) (x: t b)
+  : s: t b { v s <= v x /\ v s >= v x - 1 /\ (v s > b.min ==> v s = v x - 1)} =
+  if x.repr `REPR.gt` REPR.int_to_t b.min
+  then { repr = REPR.sub x.repr 1l }
+  else x
+
+let extend (#b: bounds) (#b': bounds { b'.min <= b.min /\ b.max <= b'.max }) (x: t b)
+  : s: t b' { v s == v x } =
+  { repr = x.repr }
+
+let shrink (#b: bounds) (#b': bounds) (x: t b { b'.min <= v x /\ v x <= b'.max })
+  : s: t b' { v s == v x } =
+  { repr = x.repr }
+
+let s32r_to_u64 (#b: bounds { 0 <= b.min }) (x: t b)
+  : r: U64.t { U64.v r == v x } =
+  let r = Cast.int32_to_uint64 x.repr in
+  assert (U64.v r == v x);
+  r
+
+let s32r_to_u8 (#b: bounds { 0 <= b.min /\ b.max <= 255 }) (x: t b)
+  : r: U8.t { U8.v r == v x } =
+  let r = Cast.int32_to_uint8 x.repr in
+  assert (U8.v r == v x);
+  r
+
+let u64_to_s32r (#b: bounds) (x: U64.t { b.min <= U64.v x /\ U64.v x <= b.max }): t b =
+  // Deprecated, but this is a safe usage
+  let r = { repr = Cast.uint64_to_int32 x } in
+  assert (v r == U64.v x);
+  r
+
+let u8_to_s32r (#b: bounds) (x: U8.t { b.min <= U8.v x /\ U8.v x <= b.max }): t b =
+  let r = { repr = Cast.uint8_to_int32 x } in
+  assert (v r == U8.v x);
+  r
+
+// TODO implement remaining saturated operations...
+
+let clamp (#b: bounds) (x: REPR.t): t b =
+  let min = REPR.int_to_t b.min in
+  let max = REPR.int_to_t b.max in
+  if REPR.lt x min then { repr = min }
+  else if REPR.gt x max then { repr = max }
+  else { repr = x }
+
+let add_sat (#b1: bounds) (#b2: bounds { Int.fits (b1.min + b2.min) REPR.n /\ Int.fits (b1.max + b2.max) REPR.n }) (x: t b1) (y: t b2): t b1 =
+  let r = REPR.add x.repr y.repr in
+  clamp r
+
+// let div_underspec (a b: t min max): r: t { REPR.v b <> 0 ==> r = REPR.div a b } =
+//   if b = 0uL then 0uL else REPR.div a b
+
+// very under-specified rem: requires minimum bound to be 0 to avoid overflows like -32768/-1
+let rem_underspec (#b: bounds { b.min == 0 }) (x y: t b): t b  =
+  // refinement? { REPR.v y.repr <> 0 ==> REPR.v r.repr == REPR.v x.repr % REPR.v y.repr }
+  if y.repr <> 0l then begin
+    let r = REPR.rem x.repr y.repr in
+    { repr = r }
+  end else
+    { repr = 0l }
+
+
+let min (#b: bounds) (x y: t b): t b =
+  if REPR.lt x.repr y.repr then x else y
+
+let max (#b: bounds) (x y: t b): t b =
+  if REPR.lt x.repr y.repr then y else x
+
+#push-options "--split_queries always --fuel 1 --ifuel 0"
+
+
+(* Bit-shifting power-of-two; pow2 and Int.pow2_n are not extractable to C. *)
+let pow2_n (#b: bounds { b.min == 0 /\ b.max <= 30 }) (x: t b): t { min = 1; max = Int.pow2_n #REPR.n b.max } =
+  let shift = Cast.int32_to_uint32 x.repr in
+  Math.pow2_le_compat 30 (UInt32.v shift);
+  Math.pow2_le_compat b.max (UInt32.v shift);
+  let pow = REPR.shift_left 1l shift in
+  { repr = pow }
+
+#pop-options
+
+let pow2_minus_one (#b: bounds { b.min == 0 /\ b.max <= 30 }) (x: t b): t { min = 0; max = Int.pow2_n #REPR.n b.max - 1 } =
+  let pow = pow2_n x in
+  { repr = REPR.sub pow.repr 1l }
+
+let gt  (#b: bounds) (x y: t b): bool = REPR.gt  x.repr y.repr
+let gte (#b: bounds) (x y: t b): bool = REPR.gte x.repr y.repr
+let lt  (#b: bounds) (x y: t b): bool = REPR.lt  x.repr y.repr
+let lte (#b: bounds) (x y: t b): bool = REPR.lte x.repr y.repr
+
+(*** Infix notations *)
+// unfold let op_Plus = add_underspec
+// unfold let op_Subtraction = sub_underspec
+// unfold let op_Star = mul_underspec
+// unfold let op_Slash = div_underspec
+unfold let op_Percent (#b: bounds { b.min == 0 }) = rem_underspec #b
+// unfold let op_Hat = logxor
+// unfold let op_Amp = logand
+// unfold let op_Bar = logor
+// unfold let op_Less_Less = shift_left
+// unfold let op_Greater_Greater = shift_right
+unfold let op_Greater (#b: bounds) = gt #b
+unfold let op_Greater_Equals (#b: bounds) = gte #b
+unfold let op_Less (#b: bounds) = lt #b
+unfold let op_Less_Equals (#b: bounds) = lte #b
