example/ttcan2/Network.TTCan.Prim.U64.fst
@@ -1,0 +1,41 @@
+(* Under-specified uint64 primitives for use in Pipit;
+  Pipit doesn't support preconditions on primitives yet.
+  TODO: This should be renamed to something like UInt64Underspec
+  *)
+module Network.TTCan.Prim.U64
+
+module PSSB      = Pipit.Prim.HasStream
+
+module REPR    = FStar.UInt64
+module UInt    = FStar.UInt
+
+let t = REPR.t
+
+instance has_stream_U64: PSSB.has_stream t = {
+  ty_id = [`%REPR.t];
+  val_default = 0uL;
+}
+
+let valid (i: t): bool = UInt.fits (REPR.v i) REPR.n
+
+let div_underspec (a b: t): r: t { REPR.v b <> 0 ==> r = REPR.div a b } =
+  if b = 0uL then 0uL else REPR.div a b
+
+let rem_underspec (a b: t): r: t { REPR.v b <> 0 ==> r = REPR.rem a b }  =
+  if b = 0uL then 0uL else REPR.rem a b
+
+(*** Infix notations *)
+unfold let op_Plus = REPR.add_underspec
+unfold let op_Subtraction = REPR.sub_underspec
+unfold let op_Star = REPR.mul_underspec
+unfold let op_Slash = div_underspec
+unfold let op_Percent = rem_underspec
+unfold let op_Hat = REPR.logxor
+unfold let op_Amp = REPR.logand
+unfold let op_Bar = REPR.logor
+// unfold let op_Less_Less = REPR.shift_left
+// unfold let op_Greater_Greater = shift_right
+unfold let op_Greater = REPR.gt
+unfold let op_Greater_Equals = REPR.gte
+unfold let op_Less = REPR.lt
+unfold let op_Less_Equals = REPR.lte
