example/ttcan2/Network.TTCan.Types.Config.fst
@@ -1,0 +1,35 @@
+(* Configuration for a specific TTCan node.
+  The config type contains the settings and trigger array, as well as proofs
+  that the trigger array can be scheduled.
+*)
+module Network.TTCan.Types.Config
+
+open Network.TTCan.Types.Base
+open Network.TTCan.Types.Triggers
+
+module Subrange   = Network.TTCan.Prim.S32R
+
+
+noeq
+type config = {
+  initial_ref_offset: ref_offset;
+  master_index: option master_index;
+  tx_enable_window: tx_enable_window; // spec says upper limit is 16 - why 16?
+  cycle_count_max: cycle_index;
+
+
+  (*^8.3 When a failed time master reconnects to the system with active time-triggered communication, it shall wait until it is synchronised to the network before attempting to become time master again. *)
+  (* This requirement is somewhat vague and seems to introduce a potential deadlock if all masters had previously failed. I have implemented it by specifying a delay to stop transmissions after a severe failure occurs. *)
+  severe_error_ref_cooldown: ntu_config;
+
+  triggers: triggers;
+  // TODO: trigger validity check: space between them;
+
+  expected_tx_triggers: trigger_count;
+}
+
+let config_master_enable (cfg: config): bool = Some? cfg.master_index
+let config_master_index (cfg: config): master_index =
+  match cfg.master_index with
+  | None -> Subrange.s32r 0
+  | Some ix -> ix
